examples/xlrup_checker/xlrupScript.sml
@@ -943,44 +943,80 @@ Definition conv_xor_mv_def:
   conv_rawxor mv (MAP conv_lit x)
 End
 
+Definition get_name_def:
+  get_name (t,n) (v:num) =
+  case lookup v t of
+    NONE => (n, (insert v n t, n+(1:num)))
+  | SOME m => (m, (t,n))
+End
+
+Definition ren_int_ls_def:
+  (ren_int_ls tn [] (acc:int list) = (REVERSE acc, tn)) ∧
+  (ren_int_ls tn (i::is) acc =
+    let v = Num (ABS i) in
+    let (m,tn) = get_name tn v in
+    let vv = if i < (0:int) then -&m else &m in
+    ren_int_ls tn is (vv::acc))
+End
+
+Definition ren_lit_ls_def:
+  (ren_lit_ls tn [] (acc:lit list) = (REVERSE acc, tn)) ∧
+  (ren_lit_ls tn (i::is) acc =
+    case i of
+      Pos v =>
+      let (m,tn) = get_name tn v in
+        ren_lit_ls tn is (Pos m::acc)
+    | Neg v =>
+      let (m,tn) = get_name tn v in
+        ren_lit_ls tn is (Neg m::acc))
+End
+
+(* note: in CFromX, we remap the clause for checking against XORs but store the original clause  *)
 Definition check_xlrup_def:
-  check_xlrup xorig xlrup cfml xfml def =
+  check_xlrup xorig xlrup cfml xfml tn def =
   case xlrup of
-    Del cl => SOME (FOLDL (\a b. delete b a) cfml cl, xfml, def)
+    Del cl =>
+    SOME (FOLDL (\a b. delete b a) cfml cl, xfml, tn, def)
   | RUP n C i0 =>
     if is_rup cfml i0 C then
-      SOME (insert n C cfml, xfml, def)
+      SOME (insert n C cfml, xfml, tn, def)
     else NONE
   | XOrig n rX =>
     if MEM rX xorig
     then
-      let X = conv_xor_mv def rX in
-      SOME (cfml, insert n X xfml, MAX def (strlen X))
+      let (mX,tn) = ren_lit_ls tn rX [] in
+      let X = conv_xor_mv def mX in
+      SOME (cfml, insert n X xfml, tn, MAX def (strlen X))
     else NONE
   | XAdd n rX i0 i1 =>
-    let X = conv_rawxor def rX in
+    let (mX,tn) = ren_int_ls tn rX [] in
+    let X = conv_rawxor def mX in
     if is_xor def xfml i0 cfml i1 X then
-      SOME (cfml, insert n X xfml, MAX def (strlen X))
+      SOME (cfml, insert n X xfml, tn, MAX def (strlen X))
     else NONE
-  | XDel xl => SOME (cfml, FOLDL (\a b. delete b a) xfml xl, def)
+  | XDel xl =>
+      SOME (cfml, FOLDL (\a b. delete b a) xfml xl, tn, def)
   | CFromX n C i0 =>
-    if is_cfromx def xfml i0 C then
-      SOME (insert n C cfml, xfml, def)
+    let (mC,tn) = ren_int_ls tn C [] in
+    if is_cfromx def xfml i0 mC then
+      SOME (insert n C cfml, xfml, tn, def)
     else NONE
   | XFromC n rX i0 =>
     if is_xfromc cfml i0 rX then
-      let X = conv_rawxor def rX in
-      SOME (cfml, insert n X xfml, MAX def (strlen X))
+      let (mX,tn) = ren_int_ls tn rX [] in
+      let X = conv_rawxor def mX in
+      SOME (cfml, insert n X xfml, tn, MAX def (strlen X))
     else NONE
 End
 
 Definition check_xlrups_def:
-  (check_xlrups xorig [] cfml xfml def = SOME (cfml,xfml,def)) ∧
-  (check_xlrups xorig (x::xs) cfml xfml def =
-  case check_xlrup xorig x cfml xfml def of
+  (check_xlrups xorig [] cfml xfml tn def =
+    SOME (cfml,xfml,tn,def)) ∧
+  (check_xlrups xorig (x::xs) cfml xfml tn def =
+  case check_xlrup xorig x cfml xfml tn def of
     NONE => NONE
-  | SOME (cfml',xfml',def') =>
-    check_xlrups xorig xs cfml' xfml' def')
+  | SOME (cfml',xfml',tn',def') =>
+    check_xlrups xorig xs cfml' xfml' tn' def')
 End
 
 Definition contains_emp_def:
@@ -990,10 +1026,10 @@ Definition contains_emp_def:
 End
 
 Definition check_xlrups_unsat_def:
-  check_xlrups_unsat xorig xlrups cfml xfml def =
-  case check_xlrups xorig xlrups cfml xfml def of
+  check_xlrups_unsat xorig xlrups cfml xfml tn def =
+  case check_xlrups xorig xlrups cfml xfml tn def of
     NONE => F
-  | SOME (cfml',xfml',def') => contains_emp cfml'
+  | SOME (cfml',xfml',tn'def') => contains_emp cfml'
 End
 
 (* Proofs *)
@@ -1319,10 +1355,12 @@ QED
 
 Theorem wf_cfml_check_xlrup:
   wf_cfml cfml ∧ wf_xlrup xlrup ∧
-  check_xlrup xorig xlrup cfml xfml def = SOME (cfml',xfml',def') ⇒
+  check_xlrup xorig xlrup cfml xfml tn def =
+    SOME (cfml',xfml',tn',def') ⇒
   wf_cfml cfml'
 Proof
-  rw[check_xlrup_def]>>gvs[AllCaseEqs()]
+  rw[check_xlrup_def]>>gvs[AllCaseEqs()]>>
+  rpt(pairarg_tac>>fs[])
   >-
     metis_tac[wf_cfml_delete_clauses]
   >- (
@@ -1486,14 +1524,18 @@ Proof
   metis_tac[isat_cfml_get_clauses,imp_cclause_imp]
 QED
 
+(* TODO: needs an invariant on tn and
+  how it remaps w when passing to xfml *)
 Theorem check_xlrup_sound:
   wf_xlrup xlrup ∧
-  check_xlrup xorig xlrup cfml xfml def =
-    SOME (cfml',xfml',def') ∧
+  check_xlrup xorig xlrup cfml xfml tn def =
+    SOME (cfml',xfml',tn',def') ∧
   (∀x. MEM x xorig ⇒ sat_cmsxor w x) ∧
   isat_fml w (values cfml, values xfml) ⇒
   isat_fml w (values cfml', values xfml')
 Proof
+  cheat
+  (*
   rw[check_xlrup_def]>>
   gvs[AllCaseEqs()]
   >- (* deleting clauses by ID *)
@@ -1553,20 +1595,21 @@ Proof
       (EVAL_TAC>>rw[])>>
     fs[wf_xlrup_def]>>
     drule_all is_xfromc_sound>>
-    EVAL_TAC)
+    EVAL_TAC) *)
 QED
 
 (* The main operational theorem about check_xlrups *)
 Theorem check_xlrups_sound:
-  ∀ls cfml xfml def def'.
+  ∀ls cfml xfml def def' tn tn'.
   EVERY wf_xlrup ls ∧
-  check_xlrups xorig ls cfml xfml def = SOME (cfml',xfml',def') ∧
+  check_xlrups xorig ls cfml xfml tn def =
+    SOME (cfml',xfml', tn', def') ∧
   (∀x. MEM x xorig ⇒ sat_cmsxor w x) ⇒
   (isat_fml w (values cfml, values xfml) ⇒
    isat_fml w (values cfml', values xfml'))
 Proof
   Induct>>simp[check_xlrups_def]>>
-  ntac 5 strip_tac>>
+  rw[]>>
   every_case_tac>>fs[]>>
   rw[]>>
   drule check_xlrup_sound>>
@@ -1617,7 +1660,7 @@ QED
 Theorem check_xlrups_unsat_sound:
   EVERY wf_xlrup xlrups ∧
   check_xlrups_unsat xfml xlrups
-    (build_fml cid cfml) LN def ⇒
+    (build_fml cid cfml) LN (LN,1) def ⇒
   ¬ ∃w.
     isat_cfml w (set cfml) ∧
     (∀x. MEM x xfml ⇒ sat_cmsxor w x)
@@ -1630,8 +1673,8 @@ Proof
     rw[]>>
     asm_exists_tac>>simp[isat_cclause_def])>>
   fs[]>>
-  Cases_on`r`>>drule check_xlrups_sound>>
-  disch_then drule>>
+  PairCases_on`r`>>drule check_xlrups_sound>>
+  disch_then (drule_at Any)>>
   fs[isat_fml_def,values_build_fml]>>
   simp[values_def,isat_xfml_def]>>
   metis_tac[]
